Complete revamp of reactions.

src/determinism.lean
@@ -1,11 +1,17 @@
 import data.finset
 import data.set.finite
 
+-- open classical
+-- local attribute [instance, priority 0] prop_decidable
+
 /- Reactor Primitives -/
 
 -- A reactor's state fields and ports are represented as maps from (a fixed set of) indices to
 -- (possibly absent) values. Single ports and state fields can therefore be identified by values
 -- of these maps' domains (i.e. indices).
+--
+--? It should be possible to extract the "core" of these definitions into a single definition and
+--? then just have `ports` and `state` be typealiases for that core.
 namespace reactor
 
   inductive value : Type*
@@ -13,6 +19,8 @@ namespace reactor
 
   def ports (n : ℕ) := (fin n) → (option value)
   def state (n : ℕ) := (fin n) → (option value)
+
+  def ports.absent {n : ℕ} : ports n := λ _, none
 
 end reactor
 open reactor
@@ -51,196 +59,104 @@ structure reaction (nᵢ nₒ nₛ : ℕ) :=
 
 namespace reaction
 
+  -- (1) Get R's triggers T.
+  -- (2) Coerce the elements in T to be the input type of P.
+  -- (3) Get the codomain C of (T through P).
+  -- (4) Erase the absent value (`none`) from C.
+  -- (4) If C is empty (contained nothing but the absent value), R is not triggered by P.
+  def is_triggered_by {nᵢ nₒ nₛ : ℕ} (r : reaction nᵢ nₒ nₛ) (is : ports nᵢ) : Prop :=
+    let ts : finset (fin nᵢ) := r.triggers.map ⟨λ i, ↑i, subtype.coe_injective⟩ in
+    let i : finset (option value) := ts.image is in
+    let vs := i.erase none in
+    vs.nonempty
+
+  instance {nᵢ nₒ nₛ : ℕ} (r : reaction nᵢ nₒ nₛ) (is : ports nᵢ) : decidable (is_triggered_by r is) := sorry
+
   -- A reaction is deterministic, if given equal inputs and states, running the body produces equal
   -- outputs and states. 
   -- Since a reaction's body is a function, determinism is trivially fulfilled.
-  theorem determinism {nᵢ nₒ nₛ : ℕ } (r : reaction nᵢ nₒ nₛ) (i₁ i₂ : input r.dᵢ) (s₁ s₂ : state nₛ) :
+  theorem determinism {nᵢ nₒ nₛ : ℕ} (r : reaction nᵢ nₒ nₛ) (i₁ i₂ : input r.dᵢ) (s₁ s₂ : state nₛ) :
     i₁ = i₂ ∧ s₁ = s₂ → (r.body i₁ s₁) = (r.body i₂ s₂) := 
     assume h, congr (congr_arg r.body h.left) h.right
 
 end reaction
 
-/- Reactions -/
-
-namespace reactor 
-
-  -- The `reactions` type describes a non-empty list of reactions, which are thereby given an
-  -- implicit order.
-  -- In this simplified model of reactors, precendece between reactions arises *only* from an
-  -- *explicit* ordering. The precedence *graph* of reactions therefore collapses to a *list*.
-  inductive reactions (nᵢ nₒ nₛ : ℕ)
-    | just  (r : reaction nᵢ nₒ nₛ) : reactions
-    | chain (head : reaction nᵢ nₒ nₛ) (tail : reactions) : reactions
-
-end reactor
-open reactor
-
 /- Reactor -/
 
-structure reactor {nᵢ nₒ nₛ : ℕ} :=
+structure reactor (nᵢ nₒ nₛ : ℕ) :=
   (inputs : ports nᵢ)
   (outputs : ports nₒ)
   (st : state nₛ)
-  (rs : reactions nᵢ nₒ nₛ)
+  (rs : list (reaction nᵢ nₒ nₛ))
 
 namespace reactor 
 
-  private def input_from_ports {n : ℕ} (dᵢ : finset (fin n)) (p : ports n) : input dᵢ :=
-    λ i : {d // d ∈ dᵢ}, p i
+  instance ports_to_input {n : ℕ} {dᵢ : finset (fin n)} : has_lift (ports n) (input dᵢ) :=
+    ⟨λ p, λ i : {d // d ∈ dᵢ}, p i⟩
 
-  private def ports_from_output {n : ℕ} {dₒ : finset (fin n)} (o: output dₒ) : ports n :=
-    λ i : fin n, if h : i ∈ dₒ then o ⟨i, h⟩ else none
+  instance output_to_ports {n : ℕ} {dₒ : finset (fin n)} : has_lift (output dₒ) (ports n) :=
+    ⟨λ o, λ i : fin n, if h : i ∈ dₒ then o ⟨i, h⟩ else none⟩
+
+  -- TEMPORARY (ports_to_input)
+  private def lift_ {n : ℕ} {dᵢ : finset (fin n)} : (ports n) → (input dᵢ) :=
+    λ p, λ i : {d // d ∈ dᵢ}, p i
+  -- TEMPORARY (output_to_ports)
+  private def lift_ {n : ℕ} {dₒ : finset (fin n)} : (output dₒ) → (ports n) :=
+    λ o, λ i : fin n, if h : i ∈ dₒ then o ⟨i, h⟩ else none
 
   private def merge_ports {n : ℕ} (first : ports n) (last : ports n) : ports n :=
     λ i : fin n, (last i).elim (first i) (λ v, some v)
 
-  private lemma lt_le_trans {n₁ n₂ n₃ : ℕ} : (n₁ < n₂ ∧ n₂ ≤ n₃) → n₁ < n₃ := sorry
-  private lemma fn {n₁ n₂ : ℕ} (h : n₁ ≤ n₂) : fin n₁ → fin n₂ := λ i, ⟨↑i, lt_le_trans ⟨i.is_lt, h⟩⟩
-  private lemma fn_inj {n₁ n₂ : ℕ} (h : n₁ ≤ n₂) : function.injective (fn h) := sorry
-  private lemma exp_ind {nᵢ : ℕ} (is : finset (fin nᵢ)) (n : ℕ) (h : nᵢ ≤ n) : finset (fin n) := is.map ⟨fn h, fn_inj h⟩  
+  private def run' {nᵢ nₒ nₛ : ℕ} : (ports nᵢ) → (state nₛ) → (list (reaction nᵢ nₒ nₛ)) → (ports nₒ × state nₛ)
+    | i s [] := ⟨ports.absent, s⟩ 
+    | i s (rₕ :: rₜ) := 
+      let osₕ : ports nₒ × state nₛ := 
+        if rₕ.is_triggered_by i
+        then let os := rₕ.body (lift_ i) s in ⟨(lift_ os.1), os.2⟩ 
+        else ⟨ports.absent, s⟩ in
+      let osₜ := run' i osₕ.2 rₜ in
+      ⟨merge_ports osₕ.1 osₜ.1, osₜ.2⟩
 
-  private def run' {nᵢ nₒ nₛ : ℕ} : (ports nᵢ) → (state nₛ) → (reactions nᵢ nₒ nₛ) → (ports nₒ × state nₛ)
-    | p s (reactions.just r) :=
-      let normed_trigs : finset (fin nᵢ) := finset.map (λ t, ↑t) r.triggers in
-      let vs := normed_trigs.image p in
-      if vs = ⟨none, refl⟩  
-      then let os := r.body (input_from_ports r.dᵢ p) s in 
-           ⟨ports_from_output os.1, os.2⟩ 
-      else ⟨(λ _, none), s⟩ 
-      
-    | p s (reactions.chain h t)
-      := let fos := h.body (input_from_ports h.dᵢ p) s in
-         let tps := run' p fos.2 t in
-         ⟨merge_ports (ports_from_output fos.1) tps.1, tps.2⟩ 
-
-  def run {nᵢ nₒ nₛ : ℕ} (r : @reactor nᵢ nₒ nₛ) : @reactor nᵢ nₒ nₛ :=
-     
   --? Prove some theorems about `run` to show that it has desired behavior.
+  def run {nᵢ nₒ nₛ : ℕ} (r : reactor nᵢ nₒ nₛ) : reactor nᵢ nₒ nₛ :=
+    let os := run' r.inputs r.st r.rs in
+    ⟨ports.absent, os.1, os.2, r.rs⟩ 
+
+  -- Running a single unconnected reactor is deterministic, if equal initial states lead to equal
+  -- end states.
+  -- Since `reactor.run` is a function, determinism is trivially fulfilled.
+  theorem deterministic {nᵢ nₒ nₛ : ℕ} (r₁ r₂ : reactor nᵢ nₒ nₛ) : 
+    r₁ = r₂ → run r₁ = run r₂ :=
+    assume h, congr_arg run h
 
 end reactor
 
-/--
-
-/- Reactor Precedence List -/
-
-namespace reactor
-
-  -- In this simple model of reactors, precendece between reactions arises *only* from an explicit
-  -- ordering (not reactor-internal dependencies). The precedence *graph* therefore collapses to a
-  -- *list* which codifies the order implicitly.
-  -- The list is also used as the means of collecting all of the reactions of a reactor.
-  -- An own type is chosen over `list`, to disallow empty lists.
-  inductive precedence_list
-    | single (r : reaction) : precedence_list
-    | chain (first : reaction) (later : precedence_list) : precedence_list
-
-  namespace precedence_list
-
-    -- Merges two outputs in such a way that all of the non-`ε` values of `o₁` override the values
-    -- in `o₂`.
-    --? Require proof that lengths of o1/2 are equal and equal o.
-    private def merge (o₁ o₂ : output) : output := sorry
-
-    -- Cf. `process`.
-    private def process' : (input × output × state) → (precedence_list) → (output × state)
-      | ios (single r)  := let os := r ⟨ios.1, ios.2.2⟩ in 
-                           ⟨merge os.1 ios.2.1, os.2⟩ 
-      | ios (chain f l) := let os := f ⟨ios.1, ios.2.2⟩ in
-                           let os' := process' ⟨ios.1, os.1, os.2⟩ l in
-                           ⟨merge os.1 os'.1, os'.2⟩ 
-
-    -- Basic reactions process their input directly, since they are functions. A collection 
-    -- (precedence-list) of reactions uses the following mechanism, to go from input to singular
-    -- final output.
-    -- Reactions were defined as functions that only change the state or return outputs different
-    -- from `ε`s (cf. `reaction`) *if* they consider themselves to be dependent on the given input.
-    -- In turn, to compute the result of a collection of reactions for a given input, the input can
-    -- simply be fed through the precendence list, from one reaction to the next.
-    -- If a reaction changes the state, this updated state will be passed along to the next
-    -- reaction.
-    -- If a reaction produces output, this output will be merged onto a cumulative outputs-value
-    -- that is carried along the processing-chain (cf. `process'`).
-    -- If a reaction is definitionally considered to not trigger on the given input, its output
-    -- will change neither the state- nor outputs-value that is carried along the processing-chain.
-    -- To implement this functionality, a seperate `process'` function is used, that can carry the
-    -- outputs.
-    def process : (input × state) → (precedence_list) → (output × state)
-      | is (single r)  := r is
-      | is (chain f l) := let os := f is in
-                          process' ⟨is.1, os.1, os.2⟩ l
-
-    -- A collection (precendence-list) of reactions is deterministic, if given equal inputs, the
-    -- results of processing them is equal. 
-    -- Since `process` is a function, determinism is trivially fulfilled.
-    theorem deterministic (p : precedence_list) (is₁ is₂ : input × state) : 
-      is₁ = is₂ → (process is₁ p) = (process is₂ p) :=
-      assume h : is₁ = is₂, 
-      congr (congr_arg process h) (refl p)
-
-  end precedence_list
-
-/- Sequential Processing -/
+/- Sequential -/
 
 namespace reactor
 
   namespace sequential
     
-    -- Given a list of inputs, an initial state and a collection of reactions, `process` computes the
-    -- result (state and outputs) of processing the inputs sequentially, starting in the given state.
-    -- Any outputs and changes to the state produced along the way. are captured in the resulting
-    -- list.
-    -- This is akin to `reactor.precedence_list.process`, with the difference being that (a) the
-    -- basic unit of processing is now an entire precende-list (that is used repeatedly) instead of
-    -- just single reactions and (b) the outputs are listed individually rather than merged. The 
-    -- state is passed along from iteration to iteration though, just like before.
-    def process : list input → state → precedence_list → list (output × state)
-      | []        _ _ := []
-      | (iₕ :: iₜ) s p := let os' := precedence_list.process ⟨iₕ, s⟩ p in
-                         os' :: (process iₜ os'.2 p) 
+    private def run' {nᵢ nₒ nₛ : ℕ} : (reactor nᵢ nₒ nₛ) → list (ports nᵢ) → list (ports nₒ) → (reactor nᵢ nₒ nₛ) × list (ports nₒ) 
+      | r [] o := ⟨reactor.run r, o⟩ 
+      | r (iₕ :: iₜ) o := 
+        let rₕ := reactor.run r in
+        let rₜ : (reactor nᵢ nₒ nₛ) := ⟨iₕ, ports.absent, rₕ.st, rₕ.rs⟩ in 
+        run' rₜ iₜ (o ++ [rₕ.outputs])
 
-    -- Processing a sequential input to a collection of reactions is deterministic, if given equal 
-    -- inputs, the results of processing them is equal. 
-    -- Since `process` is a function, determinism is trivially fulfilled.
-    theorem deterministic (p : precedence_list) (i₁ i₂ : list input) (s₁ s₂ : state) :
-      (i₁ = i₂ ∧ s₁ = s₂) → (process i₁ s₁ p) = (process i₂ s₂ p) :=
-      assume h : i₁ = i₂ ∧ s₁ = s₂,
-      congr (congr (congr_arg process h.left) h.right) (refl p)
+    -- The first input is already within the given reactor, and the last output will also be part
+    -- of the output reactor.
+    protected def run {nᵢ nₒ nₛ : ℕ} (r : reactor nᵢ nₒ nₛ) (i : list (ports nᵢ)) : (reactor nᵢ nₒ nₛ) × list (ports nₒ) :=
+       run' r i []
+
+    -- Passing a finite sequence of inputs through a single unconnected reactor is deterministic,
+    -- if equal sequences lead to equal outputs and end states.
+    -- Since `reactor.sequence.run` is a function, determinism is trivially fulfilled.
+    theorem deterministic {nᵢ nₒ nₛ : ℕ} (r : reactor nᵢ nₒ nₛ) (i₁ i₂ : list (ports nᵢ)) : 
+      i₁ = i₂ → (sequential.run r i₁) = (sequential.run r i₂) :=
+      assume h, congr (congr_arg sequential.run (refl r)) h 
 
   end sequential
-
-end reactor
-
-/- Reactor -/
-
--- At any given time a reactor has values (or lack thereof via `ε`) for its input and output ports
--- as well as its state. The processing of values is performed by its reactions, which should only
--- ever receive the reactor's own input values and state as input. The result of processing should
--- only ever be written back to the reactor itself.
-structure old_reactor :=
-  (input_count : ℕ)
-  (output_count : ℕ)
-  («input» : vector value input_count)
-  («output» : vector value output_count)
-  («state» : state)
-  (reactions : precedence_list)
-
-namespace reactor 
-
-  -- Processing a computation for a single unconnected reactor consists of (1) processing its input
-  -- and state through its reactions (2) writing the resulting output and state back to the reactor
-  -- and (3) wiping the reactor's input (setting them all to `ε`).
-  def process (r : reactor) : reactor :=
-    let os := precedence_list.process ⟨r.input, r.state⟩ r.reactions in
-    let i' := sorry in -- Make a list of `r.input.length` many `ε`s.
-    ⟨i', os.1, os.2, r.reactions⟩ 
-
-  -- Processing a computation of a single unconnected reactor is deterministic, if given equal
-  -- inputs, the resulting reactors are equal. 
-  -- Since `process` is a function, determinism is trivially fulfilled.
-  theorem deterministic (r₁ r₂ : reactor) : 
-    r₁ = r₂ → process r₁ = process r₂ :=
-    assume h : r₁ = r₂,
-    congr_arg process h
 
 end reactor
 
@@ -248,12 +164,26 @@ end reactor
 
 namespace reactor 
 
+  namespace network
+
+    class node :=
+      (nᵢ nₒ : ℕ)
+      (inputs : ports nᵢ)
+      (outputs : ports nₒ)
+      -- (run : node → node)
+
+    -- Reactors are nodes.
+    instance {nᵢ nₒ nₛ : ℕ} {r : reactor nᵢ nₒ nₛ} : node := ⟨nᵢ, nₒ, r.inputs, r.outputs⟩
+
+  end network
+  open network
+
   -- By defining the `reactors` as a list instead of a set, we remove the need for identifiers and
   -- use the index into the list as a reactor's identifier.
-  structure network { rc : ℕ } :=
-    (reactors : vector reactor rc)
+  structure network {c : ℕ} :=
+    (nodes : vector node c)
     --? have this be a digraph of (ℕ × ℕ) instead (where each vertex can have at most one incoming edge)
-    (connections (si di : fin reactors.length) : (fin (vector.nth reactors si).output_count) → (fin (vector.nth reactors di).input_count)) 
+    (connections (si di : fin nodes.length) : (fin (vector.nth nodes si).output_count) → (fin (vector.nth nodes di).input_count)) 
 
   namespace network
 
@@ -268,5 +198,3 @@ namespace reactor
   end network
 
 end reactor
-
--/
